\documentclass[11pt]{amsart}
\usepackage{geometry}                % See geometry.pdf to learn the layout options. There are lots.
\geometry{letterpaper}                   % ... or a4paper or a5paper or ... 
%\geometry{landscape}                % Activate for for rotated page geometry
%\usepackage[parfill]{parskip}    % Activate to begin paragraphs with an empty line rather than an indent
\usepackage{graphicx}
\usepackage{amssymb}
\usepackage{epstopdf}
\DeclareGraphicsRule{.tif}{png}{.png}{`convert #1 `dirname #1`/`basename #1 .tif`.png}
\input{../tex/defs}

\title{Floor and ceiling and fractional part}
\author{The Author}
%\date{}                                           % Activate to display a given date or no date

\begin{document}
\maketitle
%\section{}
%\subsection{}

% floor/ceil in defs.tex
$\floor{x}$, $\ceil{x}$, $\{x\}$

$x = \lfloor x \rfloor + \{x\}$


$
\floor{a + b} = \ldots
$ ??


$$
0 \le \{a\} < 1  \text{ and } 0 \le \{b\} < 1  \text{ so } 0 \le \{a\} + \{b\} < 2
$$

$\{a + b\} = \{a\} + \{b\}$ if $\{a\} + \{b\} < 1$

$\{a + b\} = \{a\} + \{b\} -1 $ if $\{a\} + \{b\} \ge 1$

$$
\{a + b\} =
\begin{cases}
\{a\} + \{b\} & \text{ if } \{a\} + \{b\} < 1 \\
\{a\} + \{b\} -1  & \text{ if } \{a\} + \{b\} \ge 1 \\
\end{cases}
$$

$$
\floor{a+b} = a + b - \{a + b\}
$$

$$
\floor{a+b} = 
\begin{cases}
a + b - \{a\} - \{b\} & \text{ if } \{a\} + \{b\} < 1 \\
a + b - \{a\} - \{b\}  + 1  & \text{ if } \{a\} + \{b\} \ge 1 \\
\end{cases}
$$

$$
\floor{a+b} = 
\begin{cases}
\floor{a} + \floor{b} & \text{ if } \{a\} + \{b\} < 1 \\
\floor{a} + \floor{b}  + 1  & \text{ if } \{a\} + \{b\} \ge 1 \\
\end{cases}
$$

What about $\floor{a -b}$?



$$
\{a - b\} = \{a\} - \{b\} \text{ if } \{b\} \le \{a\}
$$

$$
\{a - b\} = 1 - (\{b\} - \{a\}) \text{ if } \{b\} > \{a\}
$$

If $\{b\} \le \{a\}$:
$$
\begin{aligned}
\floor{a - b} &= a - b - \{a - b\}
\\
& = a - b - (\{a\} - \{b\})
\\
& = a  - \{a\} - (b - \{b\})
\\
& = \floor{a} - \floor{b}
\end{aligned}
$$

If $\{b\} > \{a\}$:
$$
\begin{aligned}
\floor{a - b} &= a - b - \{a - b\}
\\
& = a - b - ( 1 - \{b\} + \{a\})
\\
& = a  - \{a\} - (b - \{b\}) - 1
\\
& = \floor{a} - \floor{b} - 1
\end{aligned}
$$






\end{document}  